Remove parser_kind

examples/miniparse/MiniParse.Spec.Base.fst
@@ -218,322 +218,25 @@ let no_lookahead_ext
   ))
 = Classical.forall_intro_2 (fun b1 -> Classical.move_requires (no_lookahead_on_ext p1 p2 b1))
 
-
-(** A parser that always consumes all its input *)
-
-let consumes_all
-  (#t: Type0)
-  (p: bare_parser t)
-: GTot Type0
-= forall (b: bytes) . Some? (bparse p b) ==> (
-    let (Some (_, len)) = bparse p b in
-    Seq.length b == len
-  )
-
-let injective_consumes_all_no_lookahead_weak
-  (#t: Type0)
-  (p: bare_parser t)
-: Lemma
-  (requires (
-    injective p /\
-    consumes_all p
-  ))
-  (ensures (
-    no_lookahead_weak p
-  ))
-= ()
-
-(** Parsing data of bounded size *)
-
-let parses_at_least
-  (sz: nat)
-  (#t: Type0)
-  (f: bare_parser t)
-: GTot Type0
-= forall (s: bytes) .
-  Some? (bparse f s) ==> (
-    let (_, consumed) = Some?.v (bparse f s) in
-    sz <= (consumed <: nat)
-  )
-
-let parses_at_least_0
-  (#t: Type0)
-  (f: bare_parser t)
-: Lemma
-  (parses_at_least 0 f)
-= ()
-
-let parses_at_least_le
-  (sz sz': nat)
-  (#t: Type0)
-  (f: bare_parser t)
-: Lemma
-  (requires (
-    parses_at_least sz f /\
-    sz' <= sz
-  ))
-  (ensures (
-    parses_at_least sz' f
-  ))
-= ()
-
-
-(** A parser that always consumes at least one byte.
-
-A list can be serialized only if the parser for elements always
-consumes at least one byte. Anyway, since we require such a parser to
-have the prefix property, this is always true except for the parser
-for empty data.
-
-*)
-
-let nonempty_strong_parser_consumes_at_least_one_byte
-  (#t: Type0)
-  (p: bare_parser t)
-  (x: bytes)
-: Lemma
-  (requires (
-    no_lookahead_weak p /\
-    no_lookahead p /\
-    injective p /\ (
-    let px = bparse p x in
-    Some? px /\ (
-    let (Some (_, len)) = px in
-    len > 0
-  ))))
-  (ensures (
-    parses_at_least 1 p
-  ))
-= let prf
-    (x' : bytes)
-  : Lemma
-    (requires (Some? (bparse p x')))
-    (ensures (
-      let px' = bparse p x' in
-      Some? px' /\ (
-      let (Some (_, len')) = px' in
-      len' > 0
-    )))
-  = let (Some (_, len')) = bparse p x' in
-    if len' > 0
-    then ()
-    else begin
-      assert (no_lookahead_weak_on p x' Seq.createEmpty);
-      assert (no_lookahead_on p Seq.createEmpty x);
-      assert (no_lookahead_on_precond p Seq.createEmpty x);
-      assert (no_lookahead_on_postcond p Seq.createEmpty x);
-      assert (injective_precond p Seq.createEmpty x);
-      assert (injective_postcond p Seq.createEmpty x)
-    end
-  in
-  Classical.forall_intro (Classical.move_requires prf)
-
-
-let parses_at_most
-  (sz: nat)
-  (#t: Type0)
-  (f: bare_parser t)
-: GTot Type0
-= forall (s: bytes) .
-  Some? (bparse f s) ==> (
-    let (_, consumed) = Some?.v (bparse f s) in
-    sz >= (consumed <: nat)
-  )
-
-let is_constant_size_parser
-  (sz: nat)
-  (#t: Type0)
-  (f: bare_parser t)
-: GTot Type0
-= forall (s: bytes) .
-  Some? (bparse f s) ==> (
-    let (_, consumed) = Some?.v (bparse f s) in
-    sz == (consumed <: nat)
-  )
-
-let is_constant_size_parser_equiv
-  (sz: nat)
-  (#t: Type0)
-  (f: bare_parser t)
-: Lemma
-  (is_constant_size_parser sz f <==> (parses_at_least sz f /\ parses_at_most sz f))
-= ()
-
-let is_total_constant_size_parser
-  (sz: nat)
-  (#t: Type0)
-  (f: bare_parser t)
-: GTot Type0
-= forall (s: bytes) . {:pattern (f s) }
-  (Seq.length s < sz) == (None? (f s))
-
-type parser_subkind =
-  | ParserStrong
-
-let parser_subkind_prop (k: parser_subkind) (#t: Type0) (f: bare_parser t) : GTot Type0 =
-  match k with
-  | ParserStrong ->
-    no_lookahead f
-
-type parser_kind' = {
-  parser_kind_low: nat;
-  parser_kind_high: option nat;
-  parser_kind_subkind: option parser_subkind;
-}
-
-let parser_kind = (x: parser_kind' {
-  Some? x.parser_kind_high ==> x.parser_kind_low <= Some?.v x.parser_kind_high
-})
-
-inline_for_extraction
-let strong_parser_kind (lo hi: nat) : Pure parser_kind
-  (requires (lo <= hi))
-  (ensures (fun _ -> True))
-= {
-    parser_kind_low = lo;
-    parser_kind_high = Some hi;
-    parser_kind_subkind = Some ParserStrong;
-  }
-
-let parser_kind_prop (#t: Type0) (k: parser_kind) (f: bare_parser t) : GTot Type0 =
-  no_lookahead_weak f /\
-  injective f /\
-  parses_at_least k.parser_kind_low f /\
-  (Some? k.parser_kind_high ==> (parses_at_most (Some?.v k.parser_kind_high) f)) /\
-  (Some? k.parser_kind_subkind ==> parser_subkind_prop (Some?.v k.parser_kind_subkind) f)
-
-let parser_kind_prop_ext
-  (#t: Type0)
-  (k: parser_kind)
-  (f1 f2: bare_parser t)
-: Lemma
-  (requires (forall (input: bytes) . bparse f1 input == bparse f2 input))
-  (ensures (parser_kind_prop k f1 <==> parser_kind_prop k f2))
-= no_lookahead_ext f1 f2;
-  no_lookahead_weak_ext f1 f2;
-  injective_ext f1 f2
-
 noeq
 type parser
-  (k: parser_kind)
   (t: Type0)
-= | Parser : (f: bare_parser t { parser_kind_prop k f } ) -> parser k t
-
-let get_parser_kind
-  (#k: parser_kind)
-  (#t: Type0)
-  (p: parser k t)
-: Tot parser_kind
-= k
+= | Parser : (f: bare_parser t {
+    no_lookahead_weak f /\
+    injective f /\
+    no_lookahead f
+  } ) -> parser t
 
 (* AR: see bug#1349 *)
-unfold let coerce_to_bare_parser (t:Type0) (k2:parser_kind) (p:parser k2 t)
+unfold let coerce_to_bare_parser (t:Type0) (p:parser t)
   :Tot (bare_parser t) = Parser?.f p
 
 let parse
-  (#k: parser_kind)
   (#t: Type0)
-  (p: parser k t)
+  (p: parser t)
   (input: bytes)
 : GTot (option (t * consumed_length input))
-= bparse (coerce_to_bare_parser _ _ p) input
-
-let parser_kind_prop_intro
-  (k: parser_kind)
-  (#t: Type0)
-  (f: parser k t)
-: Lemma
-  (parser_kind_prop k (coerce_to_bare_parser _ _ f))
-= ()
-
-let is_weaker_than
-  (k1 k2: parser_kind)
-: GTot Type0
-= k1.parser_kind_low <= k2.parser_kind_low /\
-  (Some? k1.parser_kind_high ==> (
-    Some? k2.parser_kind_high /\
-    Some?.v k2.parser_kind_high <= Some?.v k1.parser_kind_high
-  )) /\
-  (Some? k1.parser_kind_subkind ==> k1.parser_kind_subkind == k2.parser_kind_subkind)
-
-unfold
-let weaken (k1: parser_kind) (#k2: parser_kind) (#t: Type0) (p2: parser k2 t) : Pure (parser k1 t)
-  (requires (k1 `is_weaker_than` k2))
-  (ensures (fun _ -> True))
-= (Parser (coerce_to_bare_parser t k2 p2) <: (parser k1 t))
-
-#reset-options
-
-// inline_for_extraction
-unfold
-let strengthen (k: parser_kind) (#t: Type0) (f: bare_parser t) : Pure (parser k t)
-  (requires (parser_kind_prop k f))
-  (ensures (fun _ -> True))
-= Parser f
-
-let glb
-  (k1 k2: parser_kind)
-: Pure parser_kind
-  (requires True)
-  (ensures (fun k ->
-    k `is_weaker_than` k1 /\
-    k `is_weaker_than` k2 /\
-    (forall k' . (k' `is_weaker_than` k1 /\ k' `is_weaker_than` k2) ==> k' `is_weaker_than` k)
-  ))
-= {
-    parser_kind_low = (if k1.parser_kind_low < k2.parser_kind_low then k1.parser_kind_low else k2.parser_kind_low);
-    parser_kind_high = (
-      if Some? k1.parser_kind_high && Some? k2.parser_kind_high
-      then if Some?.v k2.parser_kind_high < Some?.v k1.parser_kind_high
-	   then k1.parser_kind_high
-	   else k2.parser_kind_high
-      else None
-    );
-    parser_kind_subkind = if k1.parser_kind_subkind = k2.parser_kind_subkind then k1.parser_kind_subkind else None
-  }
-
-let default_parser_kind : (x: parser_kind {
-  forall (t: Type0) (p: bare_parser t) .
-  (no_lookahead_weak p /\ injective p) ==> parser_kind_prop x p
-})
-= {
-    parser_kind_low = 0;
-    parser_kind_high = None;
-    parser_kind_subkind = None;
-  }
-
-#set-options "--max_fuel 8 --max_ifuel 8"
-
-module L = FStar.List.Tot
-
-let rec glb_list_of
-  (#t: eqtype)
-  (f: (t -> Tot parser_kind))
-  (l: list t)
-: Pure parser_kind
-  (requires True)
-  (ensures (fun k ->
-    (forall kl . L.mem kl l ==> k `is_weaker_than` (f kl)) /\
-    (forall k' . (Cons? l /\ (forall kl . L.mem kl l ==> k' `is_weaker_than` (f kl))) ==> k' `is_weaker_than` k)
-  ))
-= match l with
-  | [] -> default_parser_kind
-  | [k] -> f k
-  | k1 :: q ->
-    let k' = glb_list_of f q in
-    glb (f k1) k'
-
-#reset-options
-
-let glb_list
-  (l: list parser_kind)
-: Pure parser_kind
-  (requires True)
-  (ensures (fun k ->
-    (forall kl . L.mem kl l ==> k `is_weaker_than` kl) /\
-    (forall k' . (Cons? l /\ (forall kl . L.mem kl l ==> k' `is_weaker_than` kl)) ==> k' `is_weaker_than` k)
-  ))
-= glb_list_of id l
+= bparse (coerce_to_bare_parser _ p) input
 
 (* Coercions *)
 
@@ -550,10 +253,9 @@ let coerce
 unfold
 let coerce_parser
   (t2: Type0)
-  (#k: parser_kind)
   (#t1: Type0)
-  (p: parser k t1)
-: Pure (parser k t2)
+  (p: parser t1)
+: Pure (parser t2)
   (requires (t2 == t1))
   (ensures (fun _ -> True))
 = p
@@ -567,30 +269,26 @@ let bare_serializer
 = t -> GTot bytes
 
 let serializer_correct
-  (#k: parser_kind)
   (#t: Type0)
-  (p: parser k t)
+  (p: parser t)
   (f: bare_serializer t)
 : GTot Type0
 = forall (x: t) . parse p (f x) == Some (x, Seq.length (f x))
 
 let serializer_correct_ext
-  (#k1: parser_kind)
   (#t1: Type0)
-  (p1: parser k1 t1)
+  (p1: parser t1)
   (f: bare_serializer t1)
-  (#k2: parser_kind)
   (#t2: Type0)
-  (p2: parser k2 t2)
+  (p2: parser t2)
 : Lemma
   (requires (t1 == t2 /\ (forall (input: bytes) . parse p1 input == parse p2 input)))
   (ensures (serializer_correct p1 f <==> serializer_correct p2 f))
 = ()
 
 let serializer_complete
-  (#k: parser_kind)
   (#t: Type0)
-  (p: parser k t)
+  (p: parser t)
   (f: bare_serializer t)
 : GTot Type0
 = forall (s: bytes) .
@@ -600,9 +298,8 @@ let serializer_complete
   )
 
 let serializer_correct_implies_complete
-  (#k: parser_kind)
   (#t: Type0)
-  (p: parser k t)
+  (p: parser t)
   (f: bare_serializer t)
 : Lemma
   (requires (serializer_correct p f))
@@ -617,39 +314,34 @@ let serializer_correct_implies_complete
       f x == Seq.slice s 0 len
     )))
   = let (Some (x, len)) = parse p s in
-    assert (no_lookahead_weak_on (coerce_to_bare_parser _ _ p) (f x) s);
-    assert (injective_precond (coerce_to_bare_parser _ _ p) (f x) s);
-    assert (injective_postcond (coerce_to_bare_parser _ _ p) (f x) s)
+    assert (no_lookahead_weak_on (coerce_to_bare_parser _ p) (f x) s);
+    assert (injective_precond (coerce_to_bare_parser _ p) (f x) s);
+    assert (injective_postcond (coerce_to_bare_parser _ p) (f x) s)
   in
   Classical.forall_intro (Classical.move_requires prf)
 
 noeq
 type serializer
-  (#k: parser_kind)
   (#t: Type0)
-  (p: parser k t)
-// : Tot Type0
+  (p: parser t)
 = | Serializer : (f: bare_serializer t { serializer_correct p f } ) -> serializer p
 
 unfold
 let coerce_serializer
   (t2: Type0)
-  (#k: parser_kind)
   (#t1: Type0)
-  (#p: parser k t1)
+  (#p: parser t1)
   (s: serializer p)
   (u: unit { t2 == t1 } )
 : Tot (serializer (coerce_parser t2 p))
 = s
 
 let serialize_ext
-  (#k1: parser_kind)
   (#t1: Type0)
-  (p1: parser k1 t1)
+  (p1: parser t1)
   (s1: serializer p1)
-  (#k2: parser_kind)
   (#t2: Type0)
-  (p2: parser k2 t2)
+  (p2: parser t2)
 : Pure (serializer p2)
   (requires (t1 == t2 /\ (forall (input: bytes) . parse p1 input == parse p2 input)))
   (ensures (fun _ -> True))
@@ -657,31 +349,27 @@ let serialize_ext
   Serializer (Serializer?.f s1 <: bare_serializer t2)
 
 let serialize_ext'
-  (#k1: parser_kind)
   (#t1: Type0)
-  (p1: parser k1 t1)
+  (p1: parser t1)
   (s1: serializer p1)
-  (#k2: parser_kind)
   (#t2: Type0)
-  (p2: parser k2 t2)
+  (p2: parser t2)
 : Pure (serializer p2)
-  (requires (t1 == t2 /\ k1 == k2 /\ p1 == p2))
+  (requires (t1 == t2 /\ p1 == p2))
   (ensures (fun _ -> True))
 = serialize_ext p1 s1 p2
 
 let serialize
-  (#k: parser_kind)
   (#t: Type0)
-  (#p: parser k t)
+  (#p: parser t)
   (s: serializer p)
   (x: t)
 : GTot bytes
 = Serializer?.f s x
 
 let serializer_unique
-  (#k: parser_kind)
   (#t: Type0)
-  (p: parser k t)
+  (p: parser t)
   (s1 s2: serializer p)
   (x: t)
 : Lemma
@@ -689,9 +377,8 @@ let serializer_unique
 = serializer_correct_implies_complete p (Serializer?.f s2)
 
 let serializer_injective
-  (#k: parser_kind)
   (#t: Type0)
-  (p: parser k t)
+  (p: parser t)
   (s: serializer p)
   (x1 x2: t)
 : Lemma
@@ -700,16 +387,13 @@ let serializer_injective
 = ()
 
 let serializer_parser_unique'
-  (#k1: parser_kind)
   (#t: Type0)
-  (p1: parser k1 t)
-  (#k2: parser_kind)
-  (p2: parser k2 t)
+  (p1: parser t)
+  (p2: parser t)
   (s: bare_serializer t)
   (x: bytes)
 : Lemma
   (requires (
-    k2.parser_kind_subkind == Some ParserStrong /\
     serializer_correct p1 s /\
     serializer_correct p2 s /\
     Some? (parse p1 x)
@@ -725,22 +409,18 @@ let serializer_parser_unique'
   assert (len == len');
   assert (parse p1 x' == Some (y, len'));
   assert (parse p2 x' == Some (y, len'));
-  assert (no_lookahead_on (coerce_to_bare_parser _ _ p2) x' x);
-  assert (no_lookahead_on_postcond (coerce_to_bare_parser _ _ p2) x' x);
-  assert (injective_postcond (coerce_to_bare_parser _ _ p2) x' x)
+  assert (no_lookahead_on (coerce_to_bare_parser _ p2) x' x);
+  assert (no_lookahead_on_postcond (coerce_to_bare_parser _ p2) x' x);
+  assert (injective_postcond (coerce_to_bare_parser _ p2) x' x)
 
 let serializer_parser_unique
-  (#k1: parser_kind)
   (#t: Type0)
-  (p1: parser k1 t)
-  (#k2: parser_kind)
-  (p2: parser k2 t)
+  (p1: parser t)
+  (p2: parser t)
   (s: bare_serializer t)
   (x: bytes)
 : Lemma
   (requires (
-    k1.parser_kind_subkind == Some ParserStrong /\
-    k2.parser_kind_subkind == Some ParserStrong /\
     serializer_correct p1 s /\
     serializer_correct p2 s
   ))
