examples/miniparse/MiniParse.Spec.List.fst
@@ -12,18 +12,6 @@ let nlist (n: nat) (t: Type) : Tot Type0 =
 
 unfold let mul = Prims.op_Multiply
 
-let parse_nlist_kind (n: nat) (k: parser_kind) : Tot parser_kind =
-  {
-    parser_kind_low = n `mul` k.parser_kind_low;
-    parser_kind_high = if n = 0 then Some 0 else if Some? k.parser_kind_high then Some (n `mul` Some?.v k.parser_kind_high) else None;
-    parser_kind_subkind = if n = 0 then Some ParserStrong else k.parser_kind_subkind;
-  }
-
-let rec parse_nlist_kind' (n: nat) (k: parser_kind) : GTot (k' : parser_kind { k' == parse_nlist_kind n k } ) =
-  if n = 0
-  then parse_ret_kind
-  else k `and_then_kind` parse_nlist_kind' (n - 1) k
-
 let synth_nlist (#t: Type) (n: nat) (xy: t * nlist n t) : Tot (nlist (n + 1) t) =
   let (x, y) = xy in
   x :: y
@@ -31,21 +19,11 @@ let synth_nlist (#t: Type) (n: nat) (xy: t * nlist n t) : Tot (nlist (n + 1) t) 
 let rec parse_nlist
   (n: nat)
   (#t: Type0)
-  (#k: parser_kind)
-  (p: parser k t)
-: Tot (parser (parse_nlist_kind n k) (nlist n t))
-= [@inline_let]
-  let _ : squash (parse_nlist_kind' n k == parse_nlist_kind n k) = () in
-  if n = 0
+  (p: parser t)
+: Tot (parser (nlist n t))
+= if n = 0
   then parse_ret []
   else (p `nondep_then` parse_nlist (n - 1) p) `parse_synth` (synth_nlist (n - 1))
-
-unfold
-let serialize_list_precond
-  (k: parser_kind)
-: GTot bool
-= k.parser_kind_subkind = Some ParserStrong &&
-  k.parser_kind_low > 0
 
 let synth_nlist_recip (#t: Type) (n: nat) (xy: nlist (n + 1) t) : Tot (t * nlist n t) =
   let (x :: y) = xy in
@@ -54,55 +32,42 @@ let synth_nlist_recip (#t: Type) (n: nat) (xy: nlist (n + 1) t) : Tot (t * nlist
 let rec serialize_nlist
   (n: nat)
   (#t: Type0)
-  (#k: parser_kind { serialize_list_precond k } )
-  (#p: parser k t)
+  (#p: parser t)
   (s: serializer p)
 : Tot (serializer (parse_nlist n p))
-= [@inline_let]
-  let _ : squash (parse_nlist_kind' n k == parse_nlist_kind n k) = () in
-  if n = 0
+= if n = 0
   then Serializer (fun _ -> Seq.createEmpty)
-  else serialize_synth _ (synth_nlist (n - 1)) (serialize_nondep_then _ s () _ (serialize_nlist (n - 1) s)) (synth_nlist_recip (n - 1)) ()
+  else serialize_synth _ (synth_nlist (n - 1)) (serialize_nondep_then s (serialize_nlist (n - 1) s)) (synth_nlist_recip (n - 1)) ()
 
 let serialize_nlist_nil
-  (#k: parser_kind)
   (#t: Type0)
-  (p: parser k t)
+  (p: parser t)
   (s: serializer p)
 : Lemma
-  (requires (
-    serialize_list_precond k
-  ))
   (ensures (serialize (serialize_nlist 0 s) [] == Seq.createEmpty))
 = ()
 
 #set-options "--z3rlimit 16"
 
 let serialize_list_cons
-  (#k: parser_kind)
   (#t: Type0)
   (n: nat)
-  (#p: parser k t)
+  (#p: parser t)
   (s: serializer p)
   (a: t)
   (q: nlist n t)
 : Lemma
-  (requires (
-    serialize_list_precond k
-  ))
   (ensures (
     serialize (serialize_nlist (n + 1) s) (a :: q) == Seq.append (serialize s a) (serialize (serialize_nlist n s) q)
   ))
 = ()
 
 let serialize_list_singleton
-  (#k: parser_kind)
   (#t: Type0)
-  (#p: parser k t)
+  (#p: parser t)
   (s: serializer p)
   (a: t)
 : Lemma
-  (requires (serialize_list_precond k))
   (ensures (serialize (serialize_nlist 1 s) [a] == serialize s a))
 = Seq.append_empty_r (serialize s a)
 
@@ -112,16 +77,14 @@ let list_length_append (l1:list 'a) (l2:list 'a) :
 = L.append_length l1 l2
 
 let rec serialize_list_append
-  (#k: parser_kind)
   (#t: Type0)
   (n1 n2: nat)
-  (#p: parser k t)
+  (#p: parser t)
   (s: serializer p)
   (l1: nlist n1 t)
   (l2: nlist n2 t)
 : Lemma
-  (requires (serialize_list_precond k))
-  (ensures (serialize_list_precond k /\ serialize (serialize_nlist (n1 + n2) s) (L.append l1 l2 <: nlist (n1 + n2) t) == Seq.append (serialize (serialize_nlist n1 s) l1) (serialize (serialize_nlist n2 s) l2)))
+  (ensures (serialize (serialize_nlist (n1 + n2) s) (L.append l1 l2 <: nlist (n1 + n2) t) == Seq.append (serialize (serialize_nlist n1 s) l1) (serialize (serialize_nlist n2 s) l2)))
 = match l1 with
   | a :: q ->
     serialize_list_append (n1 - 1) n2 s q l2;
