examples/miniparse/MiniParse.Spec.Int.fst
@@ -3,8 +3,6 @@ include MiniParse.Spec.Combinators
 
 module U8 = FStar.UInt8
 
-let parse_u8_kind = strong_parser_kind 1 1
-
-let parse_u8 : parser parse_u8_kind U8.t = make_total_constant_size_parser 1 U8.t (fun x -> Seq.index x 0)
+let parse_u8 : parser U8.t = make_total_constant_size_parser 1 U8.t (fun x -> Seq.index x 0)
 
 let serialize_u8 : serializer parse_u8 = Serializer (fun x -> Seq.create 1 x)
